proofs/Axioms.lean
@@ -5,6 +5,7 @@ import Statements
 #print axioms Protocol.Statements.check_C1
 #print axioms Protocol.Statements.check_S11_fresh
 #print axioms Protocol.Statements.check_S2_S11_check
+#print axioms Protocol.Statements.check_S29_route
 #print axioms Protocol.Statements.check_S6_level
 #print axioms Protocol.Statements.check_S6_answer
 #print axioms Protocol.Statements.check_S15_popup
